almost prove properness wrt eutt for sbuter

src/Typing_new.v
@@ -32,9 +32,19 @@ From Paco Require Import
 
 Import ITreeNotations.
 
-Section bisim.
+Import SumNotations.
+Open Scope sum_scope.
 
-  (** * `sceE` and `CompM` **)
+Inductive isTauF {E R} : itree' E R -> Prop :=
+| isTau_tau {t} : isTauF (TauF t).
+Hint Constructors isTauF : core.
+
+Definition isTau {E R} (t : itree E R) := isTauF (observe t).
+
+Definition isTauF_dec {E R} (t : itree' E R) : isTauF t \/ ~ isTauF t.
+Proof. destruct t; [ right | left | right ]; easy. Qed.
+
+Section bisim.
 
   Variant modifyE C : Type -> Type :=
   | Modify : forall (f : C -> C), modifyE C C.
@@ -47,6 +57,7 @@ Section bisim.
 
   Definition TPred S R := CompM S R -> S -> Prop.
   Definition TPred' S R := CompM' S R -> S -> Prop.
+
 
   (** * `no_errors` **)
 
@@ -107,14 +118,15 @@ Section bisim.
       auto_inj_pair2; subst; eauto.
   Qed.
 
+
   (** * `steps` and `step` **)
 
   (* The proposition that an itree has a next step *)
 
   Inductive stepsF {S R} : TPred' S R :=
   | steps_tau t s : stepsF (TauF t) s
-  | steps_modify f k s : stepsF (VisF (subevent _ (Modify f)) k) s
-  | steps_choice k s : stepsF (VisF (subevent _ Or) k) s.
+  | steps_modify f k s : stepsF (VisF (|Modify f|) k) s
+  | steps_choice k s : stepsF (VisF (||Or) k) s.
   Hint Constructors stepsF : core.
 
   Definition steps {S R} : TPred S R :=
@@ -125,59 +137,102 @@ Section bisim.
 
   Inductive stepF {S R} : CompM' S R -> S -> CompM' S R -> S -> Type :=
   | step_tau t s : stepF (TauF t) s (observe t) s
-  | step_modify f k s : stepF (VisF (subevent _ (Modify f)) k) s (observe (k s)) (f s)
-  | step_choice b k s : stepF (VisF (subevent _ Or) k) s (observe (k b)) s.
+  | step_modify f k s : stepF (VisF (|Modify f|) k) s (observe (k s)) (f s)
+  | step_choice b k s : stepF (VisF (||Or) k) s (observe (k b)) s.
+  Hint Constructors stepF : core.
 
   Definition step {S R} : CompM S R -> S -> CompM S R -> S -> Type :=
     fun t s t' s' => stepF (observe t) s (observe t') s'.
   Hint Unfold step : core.
 
   (* If `steps t s` then there exists a step from `(t,s)` *)
-  Lemma steps_impl_step {S R} (t : CompM S R) s :
-    steps t s -> exists t' s', inhabited (step t s t' s').
+
+  Lemma stepsF_impl_stepF {S R} (t : CompM' S R) s :
+    stepsF t s -> exists t' s', inhabited (stepF t s (observe t') s').
   Proof.
-    intro; unfold steps, step in *.
-    destruct H; repeat econstructor.
-    Unshelve. exact false.
+    destruct 1; unshelve (repeat econstructor). exact false.
   Qed.
 
+  Lemma steps_impl_step {S R} (t : CompM S R) s :
+    steps t s -> exists t' s', inhabited (step t s t' s').
+  Proof. apply stepsF_impl_stepF. Qed.
+
   (* If there exists a step from `(t,s)` then `steps t s` *)
+
+  Lemma stepF_impl_stepsF {S R} (t : CompM' S R) s t' s' :
+    stepF t s t' s' -> stepsF t s.
+  Proof. destruct 1; constructor. Qed.
+
   Lemma step_impl_steps {S R} (t : CompM S R) s t' s' :
     step t s t' s' -> steps t s.
+  Proof. apply stepF_impl_stepsF. Qed.
+
+  (* Deconstructing `step t s` *)
+
+  Lemma stepF_tau_inv {S R t t' s s'} :
+    @stepF S R (TauF t) s (observe t') s' ->
+    observe t' = observe t /\ s' = s.
+  Proof. intro; dependent destruction X; easy. Qed.
+
+  Lemma stepF_modify_inv {S R f k s t' s'} :
+    @stepF S R (VisF (|Modify f|) k) s (observe t') s' ->
+    observe t' = observe (k s) /\ s' = (f s).
+  Proof. intro; dependent destruction X; easy. Qed.
+
+  Lemma stepF_choice_inv {S R k s t' s'} :
+    @stepF S R (VisF (||Or) k) s (observe t') s' ->
+    { b | observe t' = observe (k b) /\ s' = s }.
+  Proof. intro; dependent destruction X; exists b; easy. Qed.
+
+  Lemma stepF_err {S R s t' s'} :
+    @stepF S R (observe (throw tt)) s (observe t') s' -> False.
+  Proof. inversion 1. Qed.
+
+  Lemma stepF_vis_eq2 {S R X e k1 k2 s t1' t2' s1' s2'} :
+    @stepF S R (VisF (X:=X) e k1) s (observe t1') s1' ->
+    @stepF S R (VisF (X:=X) e k2) s (observe t2') s2' ->
+    s1' = s2'.
   Proof.
-    intro; unfold step, steps in *.
-    destruct X; constructor.
+    destruct e as [? | [? | ?]]; intros;
+      dependent destruction X0; try dependent destruction X1; easy.
   Qed.
+
 
   (** * `sbuter` **)
 
-  Inductive sbuter_genF {S1 S2 R1 R2 : Type} sbuter (p : perm) (Q : R1 -> R2 -> Perms)
-                        : CompM' S1 R1 -> S1 -> CompM' S2 R2 -> S2 -> Prop :=
-  | sbuter_gen_ret r1 s1 r2 s2 :
+  Inductive sbuter_genF {S1 S2 R1 R2} sbuter p (Q : R1 -> R2 -> Perms)
+                        (t1 : CompM' S1 R1) s1 (t2 : CompM' S2 R2) s2 : Prop :=
+  | sbuter_gen_ret r1 r2 :
       pre p (s1, s2) ->
       p ∈ Q r1 r2 ->
-      sbuter_genF sbuter p Q (RetF r1) s1 (RetF r2) s2
-  | sbuter_gen_err t1 s1 k s2 :
-      sbuter_genF sbuter p Q t1 s1 (VisF (subevent _ (Throw tt)) k) s2
-  | sbuter_gen_step_l t1 s1 t2 s2 p' :
-      pre p (s1, s2) -> sep_step p p' ->
-      stepsF t1 s1 ->
+      RetF r1 = t1 -> RetF r2 = t2 ->
+      sbuter_genF sbuter p Q t1 s1 t2 s2
+  | sbuter_gen_err k :
+      pre p (s1, s2) -> (* TODO get rid of this assumption? *)
+      VisF (Throw tt|) k = t2 ->
+      sbuter_genF sbuter p Q t1 s1 t2 s2
+  | sbuter_gen_step_l p' :
+      pre p (s1, s2) ->
+      stepsF t1 s1 -> (isTauF t1 -> p = p') ->
+      sep_step p p' ->
       (forall t1' s1', stepF t1 s1 (observe t1') s1' ->
          guar p (s1, s2) (s1', s2)) ->
       (forall t1' s1', stepF t1 s1 (observe t1') s1' ->
          sbuter_genF sbuter p' Q (observe t1') s1' t2 s2) ->
       sbuter_genF sbuter p Q t1 s1 t2 s2
-  | sbuter_gen_step_r t1 s1 t2 s2 p' :
-      pre p (s1, s2) -> sep_step p p' ->
-      stepsF t2 s2 ->
+  | sbuter_gen_step_r p' :
+      pre p (s1, s2) ->
+      stepsF t2 s2 -> (isTauF t2 -> p = p') ->
+      sep_step p p' ->
       (forall t2' s2', stepF t2 s2 (observe t2') s2' ->
          guar p (s1, s2) (s1, s2')) ->
       (forall t2' s2', stepF t2 s2 (observe t2') s2' ->
          sbuter_genF sbuter p' Q t1 s1 (observe t2') s2') ->
       sbuter_genF sbuter p Q t1 s1 t2 s2
-  | sbuter_gen_step t1 s1 t2 s2 p' :
-      pre p (s1, s2) -> sep_step p p' ->
-      stepsF t1 s1 -> stepsF t2 s2 ->
+  | sbuter_gen_step p' :
+      pre p (s1, s2) ->
+      stepsF t1 s1 -> stepsF t2 s2 -> (isTauF t1 -> isTauF t2 -> p = p') ->
+      sep_step p p' ->
       (forall t1' s1', stepF t1 s1 (observe t1') s1' ->
        exists t2' s2' (_ : stepF t2 s2 (observe t2') s2'),
          guar p (s1, s2) (s1', s2') /\ sbuter p' Q t1' s1' t2' s2') ->
@@ -186,20 +241,331 @@ Section bisim.
          guar p (s1, s2) (s1', s2') /\ sbuter p' Q t1' s1' t2' s2') ->
       sbuter_genF sbuter p Q t1 s1 t2 s2.
 
+  Lemma sbuter_genF_mon {S1 S2 R1 R2} p Q t1 s1 t2 s2 r r' :
+    @sbuter_genF S1 S2 R1 R2 r p Q t1 s1 t2 s2 ->
+    (forall p Q t1 s1 t2 s2, r p Q t1 s1 t2 s2 -> r' p Q t1 s1 t2 s2 : Prop) ->
+    @sbuter_genF S1 S2 R1 R2 r' p Q t1 s1 t2 s2.
+  Proof.
+    induction 1; intros; subst; try solve [econstructor; eauto]; auto.
+    eapply sbuter_gen_step; eauto; intros.
+    - destruct (H4 t1' s1' X) as [t2' [s2' [X' [? ?]]]].
+      exists t2', s2', X'; eauto.
+    - destruct (H5 t2' s2' X) as [t1' [s1' [X' [? ?]]]].
+      exists t1', s1', X'; eauto.
+  Qed.
+
   Definition sbuter_gen {S1 S2 R1 R2} sbuter p Q :
     CompM S1 R1 -> S1 -> CompM S2 R2 -> S2 -> Prop :=
     fun t1 s1 t2 s2 => sbuter_genF sbuter p Q (observe t1) s1 (observe t2) s2.
+  Hint Unfold sbuter_gen : core.
 
   Definition sbuter {S1 S2 R1 R2} := paco6 (@sbuter_gen S1 S2 R1 R2) bot6.
 
   Lemma sbuter_gen_mon {S1 S2 R1 R2} : monotone6 (@sbuter_gen S1 S2 R1 R2).
   Proof.
     repeat intro. unfold sbuter_gen in *.
-    induction IN; subst; try solve [econstructor; eauto]; auto.
-    econstructor 5; eauto; intros.
-    - destruct (H3 t1' s1' X) as [t2' [s2' [X' [? ?]]]].
-      exists t2', s2', X'; eauto.
-    - destruct (H4 t2' s2' X) as [t1' [s1' [X' [? ?]]]].
-      exists t1', s1', X'; eauto.
+    eapply sbuter_genF_mon; eauto.
   Qed.
   Hint Resolve sbuter_gen_mon : paco.
+
+  Instance Proper_observing_paco2_sbuter_gen {S1 S2 R1 R2} r p Q :
+    Proper (observing eq ==> eq ==> observing eq ==> eq ==> iff)
+           (paco6 (@sbuter_gen S1 S2 R1 R2) r p Q).
+  Proof.
+    repeat intro; destruct H, H1.
+    split; intro; punfold H3; pfold; unfold sbuter_gen in *;
+      [ rewrite <- H, <- H0, <- H1, <- H2 | rewrite H, H0, H1, H2 ]; eauto.
+  Qed.
+
+  Instance Proper_observing_sbuter {S1 S2 R1 R2} p Q :
+    Proper (observing eq ==> eq ==> observing eq ==> eq ==> iff)
+           (@sbuter S1 S2 R1 R2 p Q).
+  Proof. apply Proper_observing_paco2_sbuter_gen. Qed.
+
+
+  (** * alternate constructors for `sbuter` **)
+
+  Definition sbuter_gen_tau_l {S1 S2 R1 R2 sbuter p Q} t1 s1 t2 s2 :
+    pre p (s1, s2) ->
+    sbuter_genF sbuter p Q (observe t1) s1 t2 s2 ->
+    @sbuter_genF S1 S2 R1 R2 sbuter p Q (TauF t1) s1 t2 s2.
+  Proof.
+    econstructor 3; intuition; try rewrite (proj1 (stepF_tau_inv X))
+                             ; now rewrite (proj2 (stepF_tau_inv X)).
+  Defined.
+
+  Definition sbuter_gen_tau_r {S1 S2 R1 R2 sbuter p Q} t1 s1 t2 s2 :
+    pre p (s1, s2) ->
+    sbuter_genF sbuter p Q t1 s1 (observe t2) s2 ->
+    @sbuter_genF S1 S2 R1 R2 sbuter p Q t1 s1 (TauF t2) s2.
+  Proof.
+    econstructor 4; intuition; try rewrite (proj1 (stepF_tau_inv X))
+                             ; now rewrite (proj2 (stepF_tau_inv X)).
+  Defined.
+
+  Definition sbuter_gen_modify_l {S1 S2 R1 R2 sbuter p Q} p' f k s1 t2 s2 :
+      pre p (s1, s2) ->
+      sep_step p p' -> guar p (s1, s2) (f s1, s2) ->
+      sbuter_genF sbuter p' Q (observe (k s1)) (f s1) t2 s2 ->
+      @sbuter_genF S1 S2 R1 R2 sbuter p Q (VisF (|Modify f|) k) s1 t2 s2.
+  Proof.
+    econstructor 3 with (p':=p'); intuition; try inv H3.
+    all: try rewrite (proj1 (stepF_modify_inv X));
+         now rewrite (proj2 (stepF_modify_inv X)).
+  Defined.
+
+  Definition sbuter_gen_modify_r {S1 S2 R1 R2 sbuter p Q} p' t1 s1 f k s2 :
+      pre p (s1, s2) ->
+      sep_step p p' -> guar p (s1, s2) (s1, f s2) ->
+      sbuter_genF sbuter p' Q t1 s1 (observe (k s2)) (f s2) ->
+      @sbuter_genF S1 S2 R1 R2 sbuter p Q t1 s1 (VisF (|Modify f|) k) s2.
+  Proof.
+    econstructor 4 with (p':=p'); intuition. try inv H3.
+    all: try rewrite (proj1 (stepF_modify_inv X));
+         now rewrite (proj2 (stepF_modify_inv X)).
+  Defined.
+
+  Definition sbuter_gen_choice_l {S1 S2 R1 R2 sbuter p Q} p' k s1 t2 s2 :
+      pre p (s1, s2) ->
+      sep_step p p' ->
+      (forall b, sbuter_genF sbuter p' Q (observe (k b)) s1 t2 s2) ->
+      @sbuter_genF S1 S2 R1 R2 sbuter p Q (VisF (||Or) k) s1 t2 s2.
+  Proof.
+    econstructor 3 with (p':=p'); intuition; try inv H2.
+    all: apply stepF_choice_inv in X; destruct X as [? []];
+         try rewrite H2; rewrite H3; easy.
+  Defined.
+
+  Definition sbuter_gen_choice_r {S1 S2 R1 R2 sbuter p Q} p' t1 s1 k s2 :
+      pre p (s1, s2) ->
+      sep_step p p' ->
+      (forall b, sbuter_genF sbuter p' Q t1 s1 (observe (k b)) s2) ->
+      @sbuter_genF S1 S2 R1 R2 sbuter p Q t1 s1 (VisF (||Or) k) s2.
+  Proof.
+    econstructor 4 with (p':=p'); intuition; try inv H2.
+    all: apply stepF_choice_inv in X; destruct X as [? []];
+         try rewrite H2; rewrite H3; easy.
+  Defined.
+
+
+  (** * basic lemmas about `sbuter` **)
+
+  Lemma sbuter_genF_pre {S1 R1 S2 R2 r p Q t1 s1 t2 s2} :
+    @sbuter_genF S1 R1 S2 R2 r p Q t1 s1 t2 s2 ->
+    pre p (s1, s2) \/ exists k, VisF (Throw tt|) k = t2.
+  Proof.
+    inversion 1; eauto.
+  Qed.
+
+  Lemma sbuter_inv_tau_l {S1 S2 R1 R2} p Q t1 s1 t2 s2 :
+    @sbuter S1 S2 R1 R2 p Q (Tau t1) s1 t2 s2 ->
+    @sbuter S1 S2 R1 R2 p Q t1 s1 t2 s2.
+  Proof.
+    intro; pfold; red; punfold H; red in H.
+    dependent induction H.
+    - destruct x; econstructor 2; eauto.
+    - destruct (H1 isTau_tau); eapply H4; constructor.
+    - econstructor 4 with (p':=p'); eauto.
+    - econstructor 4 with (p':=p'); eauto; intros.
+      + apply H2; eauto; constructor.
+      + specialize (H5 _ _ X); destruct H5 as [?t1' [?s1' [? []]]].
+        inv x; eauto.
+      + specialize (H5 _ _ X); destruct H5 as [?t1' [?s1' [? []]]].
+        inv x; rewrite H10.
+        destruct H6; [|inv H6].
+        pfold_reverse; eauto.
+  Qed.
+
+  Lemma sbuter_inv_tau_r {S1 S2 R1 R2} p Q t1 s1 t2 s2 :
+    @sbuter S1 S2 R1 R2 p Q t1 s1 (Tau t2) s2 ->
+    @sbuter S1 S2 R1 R2 p Q t1 s1 t2 s2.
+  Proof.
+    intro; pfold; red; punfold H; red in H.
+    dependent induction H.
+    - econstructor 3 with (p':=p'); eauto.
+    - destruct (H1 isTau_tau); eapply H4; constructor.
+    - econstructor 3 with (p':=p'); eauto; intros.
+      + apply H2; eauto; constructor.
+      + specialize (H4 _ _ X); destruct H4 as [?t2' [?s2' [? []]]].
+        inv x; eauto.
+      + specialize (H4 _ _ X); destruct H4 as [?t1' [?s1' [? []]]].
+        inv x; rewrite H10.
+        destruct H6; [|inv H6].
+        pfold_reverse; eauto.
+  Qed.
+
+  Lemma Proper_eutt_sbuter_l {S1 S2 R1 R2} p Q t1 t1' s1 t2 s2 :
+    t1' ≈ t1 -> @sbuter S1 S2 R1 R2 p Q t1 s1 t2 s2 ->
+                @sbuter S1 S2 R1 R2 p Q t1' s1 t2 s2.
+  Proof.
+    revert p Q t1 t1' s1 t2 s2; pcofix CIH; intros.
+    pfold; red; punfold H1; red in H1.
+    revert t1' H0; dependent induction H1; intros.
+    5: punfold H6; red in H6; dependent destruction H0; destruct x.
+    (* sbuter_gen_ret *)
+    - punfold H1; red in H1.
+      destruct x0, x.
+      dependent induction H1.
+      + destruct x; econstructor; eauto.
+      + destruct x; apply sbuter_gen_tau_l; eauto.
+    (* sbuter_gen_err *)
+    - destruct x; econstructor 2; eauto.
+    (* sbuter_gen_step_l *)
+    - punfold H6; red in H6; dependent induction H6; pclearbot.
+      all: destruct x; try destruct x0; try destruct (H1 isTau_tau); eauto.
+      3: destruct e as [e | [e | e]]; destruct e; inversion H0.
+      + inversion H0.
+      + apply sbuter_gen_tau_l; eauto.
+      + eapply sbuter_gen_modify_l; eauto.
+      + eapply sbuter_gen_choice_l; eauto.
+      + apply sbuter_gen_tau_l; eauto.
+    (* sbuter_gen_step_r *)
+    - econstructor 4; eauto.
+    (* sbuter_gen_step, step_tau *)
+    - dependent induction H6; pclearbot; try destruct x.
+      + econstructor 5 with (p':=p'); eauto; intros.
+        * inv X.
+          specialize (H4 _ _ (step_tau _ _)); destruct H4 as [?t1' [?s1' [? []]]].
+          exists t1'1, s1'0, x; split; eauto.
+          destruct H4; [|inv H4].
+          right; eapply CIH; eauto.
+          rewrite <- (observing_intros _ _ _ H8); eauto.
+        * specialize (H5 _ _ X); destruct H5 as [?t2' [?s2' [? []]]].
+          inv x.
+          exists m1, s2'0, (step_tau _ _); split; eauto.
+          destruct H5; [|inv H5].
+          right; eapply (CIH _ _ t2'0); eauto.
+          rewrite <- (observing_intros _ _ _ H9); eauto.
+      + eapply sbuter_gen_tau_l; eauto.
+      + eapply IHeqitF; eauto.
+        admit. (* Hunh? Why?? *)
+    (* sbuter_gen_step, step_modify *)
+    - dependent induction H6; pclearbot; try destruct x.
+      + econstructor 5 with (p':=p'); eauto; intros.
+        * inversion H0.
+        * apply stepF_modify_inv in X; destruct X; subst.
+          specialize (H4 _ _ (step_modify _ _ _)); destruct H4 as [?t2' [?s2' [? []]]].
+          exists t2', s2', x; split; eauto.
+          destruct H6; [|inv H6].
+          right; eapply CIH; eauto.
+          rewrite (observing_intros _ _ _ H0); eauto.
+        * specialize (H5 _ _ X); destruct H5 as [?t1' [?s1' [? []]]].
+          apply stepF_modify_inv in x; destruct x; subst.
+          exists (k1 s), (f s), (step_modify _ _ _); split; eauto.
+          destruct H5; [|inv H5].
+          right; eapply (CIH _ _ t1'0); eauto.
+          rewrite (observing_intros _ _ _ H6); eauto.
+      + eapply sbuter_gen_tau_l; eauto.
+    (* sbuter_gen_step, step_choice *)
+    - dependent induction H6; pclearbot; try destruct x.
+      + econstructor 5 with (p':=p'); eauto; intros.
+        * inversion H0.
+        * apply stepF_choice_inv in X; destruct X as [b []]; subst.
+          specialize (H4 _ _ (step_choice b _ _)); destruct H4 as [?t2' [?s2' [? []]]].
+          exists t2', s2', x; split; eauto.
+          destruct H6; [|inv H6].
+          right; eapply CIH; eauto.
+          rewrite (observing_intros _ _ _ H0); eauto.
+        * specialize (H5 _ _ X); destruct H5 as [?t1' [?s1' [? []]]].
+          apply stepF_choice_inv in x; destruct x as [b []]; subst.
+          exists (k1 b), s, (step_choice b _ _); split; eauto.
+          destruct H5; [|inv H5].
+          right; eapply (CIH _ _ t1'0); eauto.
+          rewrite (observing_intros _ _ _ H6); eauto.
+  Admitted.
+
+  Lemma Proper_eutt_sbuter_r {S1 S2 R1 R2} p Q t1 s1 t2 t2' s2 :
+    t2' ≈ t2 -> @sbuter S1 S2 R1 R2 p Q t1 s1 t2 s2 ->
+                @sbuter S1 S2 R1 R2 p Q t1 s1 t2' s2.
+  Proof.
+    revert p Q t1 s1 t2 t2' s2; pcofix CIH; intros.
+    pfold; red; punfold H1; red in H1.
+    revert t2' H0; dependent induction H1; intros.
+    5: punfold H6; red in H6; dependent destruction H1; destruct x.
+    (* sbuter_gen_ret *)
+    - punfold H1; red in H1.
+      destruct x0, x.
+      dependent induction H1.
+      + destruct x; econstructor; eauto.
+      + destruct x; apply sbuter_gen_tau_r; eauto.
+    (* sbuter_gen_err *)
+    - rewrite <- (observing_intros eq (vis (Throw tt) k) _ x) in H0.
+      punfold H0; red in H0; dependent induction H0.
+      + destruct x; econstructor 2; eauto.
+      + destruct x; eapply sbuter_gen_tau_r; eauto.
+    (* sbuter_gen_step_l *)
+    - econstructor 3; eauto.
+    (* sbuter_gen_step_r *)
+    - punfold H6; red in H6; dependent induction H6; pclearbot.
+      all: destruct x; try destruct x0; try destruct (H1 isTau_tau); eauto.
+      3: destruct e as [e | [e | e]]; destruct e; inversion H0.
+      + inversion H0.
+      + apply sbuter_gen_tau_r; eauto.
+      + eapply sbuter_gen_modify_r; eauto.
+      + eapply sbuter_gen_choice_r; eauto.
+      + apply sbuter_gen_tau_r; eauto.
+    (* sbuter_gen_step, step_tau *)
+    - dependent induction H6; pclearbot; try destruct x.
+      + econstructor 5 with (p':=p'); eauto; intros.
+        * specialize (H4 _ _ X); destruct H4 as [?t2' [?s2' [? []]]].
+          inv x.
+          exists m1, s2', (step_tau _ _); split; eauto.
+          destruct H4; [|inv H4].
+          right; eapply (CIH _ _ _ _ t2'0); eauto.
+          rewrite <- (observing_intros _ _ _ H9); eauto.
+        * inv X.
+          specialize (H5 _ _ (step_tau _ _)); destruct H5 as [?t2' [?s2' [? []]]].
+          exists t2'1, s2'0, x; split; eauto.
+          destruct H5; [|inv H5].
+          right; eapply CIH; eauto.
+          rewrite <- (observing_intros _ _ _ H8); eauto.
+      + eapply sbuter_gen_tau_r; eauto.
+      + eapply IHeqitF; eauto.
+        admit. (* Hunh? Why?? *)
+    (* sbuter_gen_step, step_modify *)
+    - dependent induction H6; pclearbot; try destruct x.
+      + econstructor 5 with (p':=p'); eauto; intros.
+        * inversion H6.
+        * specialize (H4 _ _ X); destruct H4 as [?t2' [?s2' [? []]]].
+          apply stepF_modify_inv in x; destruct x; subst.
+          exists (k1 s), (f s), (step_modify _ _ _); split; eauto.
+          destruct H4; [|inv H4].
+          right; eapply (CIH _ _ _ _ t2'0); eauto.
+          rewrite (observing_intros _ _ _ H6); eauto.
+        * apply stepF_modify_inv in X; destruct X; subst.
+          specialize (H5 _ _ (step_modify _ _ _)); destruct H5 as [?t1' [?s1' [? []]]].
+          exists t1', s1', x; split; eauto.
+          destruct H6; [|inv H6].
+          right; eapply CIH; eauto.
+          rewrite (observing_intros _ _ _ H1); eauto.
+      + eapply sbuter_gen_tau_r; eauto.
+    (* sbuter_gen_step, step_choice *)
+    - dependent induction H6; pclearbot; try destruct x.
+      + econstructor 5 with (p':=p'); eauto; intros.
+        * inversion H6.
+        * specialize (H4 _ _ X); destruct H4 as [?t2' [?s2' [? []]]].
+          apply stepF_choice_inv in x; destruct x as [b []]; subst.
+          exists (k1 b), s, (step_choice b _ _); split; eauto.
+          destruct H4; [|inv H4].
+          right; eapply (CIH _ _ _ _ t2'0); eauto.
+          rewrite (observing_intros _ _ _ H6); eauto.
+        * apply stepF_choice_inv in X; destruct X as [b []]; subst.
+          specialize (H5 _ _ (step_choice b _ _)); destruct H5 as [?t1' [?s1' [? []]]].
+          exists t1', s1', x; split; eauto.
+          destruct H6; [|inv H6].
+          right; eapply CIH; eauto.
+          rewrite (observing_intros _ _ _ H1); eauto.
+  Admitted.
+
+  Instance Proper_eutt_sbuter {S1 S2 R1 R2} p Q :
+    Proper (eutt eq ==> eq ==> eutt eq ==> eq ==> iff)
+           (@sbuter S1 S2 R1 R2 p Q).
+  Proof.
+    repeat intro; split; intro; destruct H0, H2.
+    - eapply Proper_eutt_sbuter_l; [symmetry|]; eauto.
+      eapply Proper_eutt_sbuter_r; [symmetry|]; eauto.
+    - eapply Proper_eutt_sbuter_l; eauto.
+      eapply Proper_eutt_sbuter_r; eauto.
+  Qed.
+
+End bisim.
